PrimaryLogic/AD.lean
@@ -1,0 +1,25 @@
+namespace AD
+variable {α : Type u}
+
+def get (f g : List α → α) : Nat → List α × List α
+  | .zero => ([f []], [g []])
+  | .succ n =>
+    let s := get f g n
+    (f s.2 :: s.1, g s.1 :: s.2)
+
+theorem get_valid {f g : List α → α} (n : Nat) :
+    (get f g n).1 ≠ [] ∧ (get f g n).2 ≠ [] := by
+  induction n with
+  | zero => simp only [get, ne_eq, List.cons_ne_self, not_false_eq_true, and_self]
+  | succ n => simp only [get, ne_eq, reduceCtorEq, not_false_eq_true, and_self]
+
+def play (f g : List α → α) (n : Nat) : α × α :=
+  let s := get f g n
+  (s.1.head (get_valid n).1, s.2.head (get_valid n).2)
+
+def determine : Prop := ∀ p : (Nat → α × α) → Prop,
+    (∀ g, ∃ f, p (play f g)) → (∃ f, ∀ g, p (play f g))
+
+axiom determine_Bool : determine (α := Bool)
+#print axioms determine_Bool
+end AD
