PrimaryLogic/FirstOrder/Completeness.lean
@@ -23,39 +23,9 @@ theorem soundness (Γ) (φ : Formula L) : (Γ ⊢ φ) -> (Γ ∪ FOLTheory ⊨ �
   | .mp (φ := φ) (ψ := ψ) p q =>
     (soundness Γ (φ → ψ) p α M s h) (soundness Γ φ q α M s h)
 
-set_option linter.unusedDecidableInType false in
-lemma complete_iff_satisfiable [DecidablePred (Inconsistent (L := L))] :
-    (∀ Γ : Set (Formula L), Con Γ -> Satisfiable (Γ ∪ FOLTheory)) <->
-    (∀ Γ : Set (Formula L), ∀ φ : Formula L, (Γ ⊨ φ) -> (Γ ⊢ φ)) := by
-  unfold Con Consistent Satisfiable SemanticConsequence Structure.satisfies
-  constructor
-  · intro h1 Γ φ h2
-    rw [Proof.raa]
-    rcases lem <| Inconsistent (Set.insert (¬φ) Γ ∪ FOLTheory) with h5 | h5
-    · exact h5
-    · have ⟨α, M, s, h3⟩ := h1 (Γ.insert (¬φ)) h5
-      simp only [Set.mem_union, Set.insert, Set.mem_setOf_eq] at h3
-      replace h4 := h3 (¬φ)
-      simp only [true_or, FOL.mem_theory_iff, forall_const, Formula.not, Formula.interpret] at h4
-      exfalso
-      refine h4 <| h2 α M s ?_
-      intro g hg
-      exact h3 g (.inl (.inr hg))
-  · intro h1 Γ h2
-    rcases lem <| ∃ α M s, ∀ g ∈ Γ ∪ FOLTheory, Formula.interpret M s g with h' | h'
-    · exact h'
-    · simp only [not_exists, PrimaryLogic.not_forall, Set.mem_union] at h'
-      exfalso
-      apply h2
-      apply h1 Γ ⊥
-      intro α M s h
-      have ⟨x, h3, h4⟩ := h' α M s
-      exfalso; apply h4
-      rcases h3 with h3 | h3
-      · exact h x h3
-      · rw [FOL.mem_theory_iff] at h3
-        obtain ⟨a, h4⟩ := h3
-        exact h4 ▸ soundness_axiom M s a
+lemma Satisfiable_expand {Γ : Set (Formula L)} : Satisfiable Γ → Satisfiable (Γ ∪ FOLTheory) :=
+  fun ⟨α, M, s, h⟩ => ⟨α, M, s, fun g h' => Or.elim h' (h g) fun hg =>
+    Exists.elim ((FOL.mem_theory_iff g).mp hg) fun a he => he ▸ soundness_axiom M s a⟩
 
 section TermModel
 
@@ -154,4 +124,45 @@ theorem Formula.truth_lemma [DecidablePred Δ] [hk : Henkin Δ θ] (φ : Formula
         replace h' := soundness_axiom (TermModel Δ) (replace Term.var i t) a
         rwa [ha] at h'
 end TermModel
+
+section completeness
+set_option linter.unusedDecidableInType false in
+lemma complete_iff_satisfiable :
+    (∀ Γ : Set (Formula L), Con Γ -> Satisfiable (Γ ∪ FOLTheory)) <->
+    (∀ Γ : Set (Formula L), ∀ φ : Formula L, (Γ ⊨ φ) -> (Γ ⊢ φ)) := by
+  unfold Con Consistent Satisfiable SemanticConsequence Structure.satisfies
+  constructor
+  · intro h1 Γ φ h2
+    rw [Proof.raa]
+    rcases lem <| Inconsistent (Set.insert (¬φ) Γ ∪ FOLTheory) with h5 | h5
+    · exact h5
+    · have ⟨α, M, s, h3⟩ := h1 (Γ.insert (¬φ)) h5
+      simp only [Set.mem_union, Set.insert, Set.mem_setOf_eq] at h3
+      replace h4 := h3 (¬φ)
+      simp only [true_or, FOL.mem_theory_iff, forall_const, Formula.not, Formula.interpret] at h4
+      exfalso
+      refine h4 <| h2 α M s ?_
+      intro g hg
+      exact h3 g (.inl (.inr hg))
+  · intro h1 Γ h2
+    rcases lem <| ∃ α M s, ∀ g ∈ Γ ∪ FOLTheory, Formula.interpret M s g with h' | h'
+    · exact h'
+    · simp only [not_exists, PrimaryLogic.not_forall, Set.mem_union] at h'
+      exfalso
+      apply h2
+      apply h1 Γ ⊥
+      intro α M s h
+      have ⟨x, h3, h4⟩ := h' α M s
+      exfalso; apply h4
+      rcases h3 with h3 | h3
+      · exact h x h3
+      · rw [FOL.mem_theory_iff] at h3
+        obtain ⟨a, h4⟩ := h3
+        exact h4 ▸ soundness_axiom M s a
+
+variable [Encodable LF] [Encodable LP]
+
+
+
+end completeness
 end PrimaryLogic
