PrimaryLogic/Redundancy.lean
@@ -1,0 +1,110 @@
+import PrimaryLogic.Vars
+
+namespace PrimaryLogic
+variable {LF LP : Type} {L : Lang LF LP}
+section substFun
+variable [DecidableEq LF]
+
+theorem Term.fun_var_subst_distrib (i : Idx) (f : LF) (ir fr tr : Term L) : i ∉ fr.vars →
+    substFun fr f (subst i ir tr) = subst i (substFun fr f ir) (substFun fr f tr) := by
+  intro h0
+  induction tr with
+  | var j =>
+    by_cases h : i = j <;>
+    simp only [subst, h, substFun, ite_cond_eq_true, ite_cond_eq_false]
+  | app g s h =>
+    by_cases h1 : g = f
+    · simp only [subst, substFun, h1, ite_cond_eq_true]
+      apply symm
+      exact Term.subst_invariance i _ fr h0
+    · simp only [subst, substFun, h1, ite_cond_eq_false, app.injEq, heq_eq_eq, true_and]
+      funext k; exact h k
+
+lemma Term.substFun_not_mem_fvar {i : Idx} {f : LF} {fr tr : Term L} :
+    i ∉ fr.vars → i ∉ tr.vars → i ∉ (substFun fr f tr).vars := by
+  intro h0 h1
+  induction tr with
+  | var j =>
+    dsimp only [vars] at h1
+    dsimp only [substFun, vars]
+    exact h1
+  | app g s h =>
+    simp only [vars, Set.mem_iUnion, not_exists] at h1
+    dsimp only [substFun]
+    split_ifs with h2
+    · exact h0
+    · simp only [vars, Set.mem_iUnion, not_exists]
+      intro x; exact h x <| h1 x
+
+lemma Formula.substFun_not_mem_fvar {i : Idx} {f : LF} {fr : Term L} {φ : Formula L} :
+    i ∉ fr.vars → i ∉ φ.fvar → i ∉ (substFun fr f φ).fvar := by
+  intro h0 h1
+  induction φ with
+  | atom n p =>
+    simp only [substFun, fvar, Set.mem_iUnion, not_exists]
+    simp only [fvar, Set.mem_iUnion, not_exists] at h1
+    intro x; exact Term.substFun_not_mem_fvar h0 (h1 x)
+  | falsum => dsimp only [substFun, fvar, Set.notMem_empty]; trivial
+  | impl x y hx hy =>
+    simp only [substFun, fvar, Set.mem_union, not_or]
+    simp only [fvar, Set.mem_union, not_or] at h1
+    exact ⟨hx h1.left, hy h1.right⟩
+  | fall j x h' =>
+    rw [Decidable.not_imp_not] at h'
+    simp only [substFun, fvar, Set.mem_diff, not_and]
+    simp only [fvar, Set.mem_diff, not_and] at h1
+    intro h; exact h1 (h' h)
+
+lemma Formula.substFun_FreeFor {i : Idx} {f : LF} {ir fr : Term L} {φ : Formula L}
+    (hi : FreeFor i ir φ) (h : i ∉ fr.vars) (hb : fr.vars ∩ φ.bvar = ∅) :
+      FreeFor i (Term.substFun fr f ir) (Formula.substFun fr f φ) := by
+  induction φ with
+  | atom p s | falsum => dsimp only [Formula.substFun, FreeFor]
+  | impl x y hx hy =>
+    dsimp only [Formula.substFun, FreeFor]
+    have ⟨h1, h2⟩ := hi
+    simp only [bvar, Set.inter_union_distrib_left, Set.union_eq_empty] at hb
+    exact ⟨hx h1 hb.left, hy h2 hb.right⟩
+  | fall j x h' =>
+    dsimp only [Formula.substFun, FreeFor]
+    dsimp [FreeFor] at hi
+    rcases hi with h1 | h2 | ⟨h3, h4⟩
+    · left; exact h1
+    · right; left; exact Formula.substFun_not_mem_fvar h h2
+    · right; right; constructor
+      · refine Term.substFun_not_mem_fvar ?_ h3
+        unfold bvar at hb
+        by_contra
+        have h5 := Set.mem_insert j x.bvar
+        have h6 := hb ▸ Set.mem_inter this h5
+        have h7 := Set.notMem_empty j
+        contradiction
+      · simp only [bvar, Set.insert_eq, Set.inter_union_distrib_left, Set.union_eq_empty] at hb
+        exact h' h4 hb.2
+
+theorem Formula.fun_var_subst_distrib (i : Idx) (f : LF) (ir fr : Term L) (φ : Formula L)
+    (h : FreeFor i ir φ) (h1 : i ∉ fr.vars) (hb : fr.vars ∩ φ.bvar = ∅) :
+    Formula.substFun fr f (subst i ir φ h) =
+      subst i (Term.substFun fr f ir) (substFun fr f φ) (substFun_FreeFor h h1 hb) := by
+  induction φ with
+  | atom p s =>
+    simp only [subst, substFun, atom.injEq, heq_eq_eq, true_and]
+    funext k; apply Term.fun_var_subst_distrib; exact h1
+  | falsum => dsimp only [subst, substFun]
+  | impl x y hx hy =>
+    simp only [subst, substFun, impl.injEq]
+    simp only [bvar, Set.inter_union_distrib_left, Set.union_eq_empty] at hb
+    exact ⟨hx _ hb.left, hy _ hb.right⟩
+  | fall j x h' =>
+    dsimp only [subst, substFun]
+    split_ifs with h1
+    · rw [←h1]; dsimp only [substFun]
+    · simp only [substFun, fall.injEq, true_and]
+      simp only [FreeFor, h1, false_or] at h
+      simp only [bvar, Set.insert_eq, Set.inter_union_distrib_left, Set.union_eq_empty] at hb
+      rcases h with h2 | h3
+      · have := out_var_FreeFor_term ir h2
+        exact h' this hb.2
+      · exact h' h3.right hb.2
+end substFun
+end PrimaryLogic
